cesm.v
@@ -3,7 +3,7 @@ Require Import List Unicode.Utf8.
 Require Import Arith.Peano_dec.
 Require Import CpdtTactics.
 Require Import db util.
-Require Import cem.
+Require Import cem relations.
 
 Definition stack := list (closure + nat).
 
@@ -33,7 +33,7 @@ Definition replaceClosure (l:nat) (c:closure) : nat * cell → nat * cell :=
     end.
 
 Reserved Notation " c1 '→_s' c2 " (at level 50).
-Inductive step' : state → state → Prop :=
+Inductive cesm_step : transition state :=
   | Upd : ∀ Φ Υ b e e' c l s, 
   st (Φ++(l,(cl c e'))::Υ) (inr l::s) (close (lam b) e) →_s 
   st (Φ++(l,(cl (close (lam b) e) e'))::Υ) s (close (lam b) e)
@@ -43,8 +43,25 @@ Inductive step' : state → state → Prop :=
   st Φ (inl c::s) (close (lam b) e) →_s st ((f, cl c e):: Φ) s (close b f)
   | App : ∀ Φ e s n m, 
   st Φ s (close (app m n) e) →_s st Φ (inl (close n e)::s) (close m e)
-where " c1 '→_s' c2 " := (step' c1 c2).
+where " c1 '→_s' c2 " := (cesm_step c1 c2).
 
+Fixpoint transition_fold 
+  {a b : Type} {s : transition a} (st en : a) 
+  (f:forall x y, s x y → b → b) 
+  (xs:refl_trans_clos s st en) 
+  (y:b) 
+  : b :=
+  match xs with 
+  | t_refl _ _ => y 
+  | t_step _ x y' z t xs => @transition_fold a b s y' z f xs (f x y' t y) 
+  end.  
+
+Definition step_time_cost (x y : state) (s : cesm_step x y) : nat := match s with
+  | _ => 1
+  end.
+
+Definition time_cost (x y : state) (s : refl_trans_clos cesm_step x y) : nat :=
+  transition_fold x y (fun x y s b => plus (step_time_cost x y s) b) s 0.
 
 (* Step as a function *
 
