im.v
@@ -1,13 +1,90 @@
 (* Instruction Machine *)
 
-Require Import assembly util.
+Require Import assembly util relations.
 Require Import Unicode.Utf8.
+Require Import List.
+Import ListNotations.
+Require Import util.
 
 Definition Heap := Map Ptr Word.
-Definition RegisterFile := Reg → Word.
+(*
+Inductive RegisterFile := rf {
+  ip : Ptr;
+  ep : Ptr;
+  r1 : Ptr; 
+  r2 : Ptr;
+  r3 : Ptr
+}. 
 
-Inductive State := 
-  | st : RegisterFile → Program → Stack → Heap → State.
+Definition rff (r: Reg) : RegisterFile → Ptr := match r with
+  | IP => ip 
+  | EP => ep
+  | R1 => r1
+  | R2 => r2
+  | R3 => r3
+  end.
+*)
+Definition RegisterFile := Reg → Ptr.
 
-Definition I (p : Program) : State := st (λ _, 0) p nil nil. 
+Definition upd (r: Reg) (p: Ptr) (rf: RegisterFile) : RegisterFile := match r with
+  | IP => λ r, match r with | IP => p | _ => rf r end
+  | EP => λ r, match r with | EP => p | _ => rf r end
+  | R1 => λ r, match r with | R1 => p | _ => rf r end
+  | R2 => λ r, match r with | R2 => p | _ => rf r end
+  | R3 => λ r, match r with | R3 => p | _ => rf r end
+  end.
+
+Inductive State := st {
+  st_rf : RegisterFile;
+  st_p : Program;
+  st_s : Stack;
+  st_h  : Heap
+}.
+
+Definition I (p : Program) : State := st (λ r, 0) p nil nil. 
+
+Open Scope nat_scope. 
+Inductive read : RO → State → Ptr → Type :=
+  | read_reg : ∀ r s, read (RW (WR r)) s (st_rf s r)
+  | read_mem : ∀ r o rf p s h1 h2 v, 
+    read (RW (WM r o)) (st rf p s (h1++(rf r+o,v)::h2)) v
+  | read_const : ∀ c s, read (RC c) s c.
+
+Inductive write : WO → Word → State → State → Type :=
+  | write_reg : ∀ r rf p s h w, 
+    write (WR r) w (st rf p s h) (st (upd r w rf) p s h)
+  | write_mem : ∀ r o rf p s h1 h2 v w, 
+    write (WM r o) w (st rf p s (h1++(rf r+o,v)::h2)) 
+                     (st rf p s (h1++(rf r+o,w)::h2)).
+
+Inductive step_bb : BasicBlock → State → State → Type := 
+  | step_push : ∀ rf p s h ro is v sn,
+  read ro (st rf p s h) v → 
+  step_bb is (st rf p (v::s) h) sn → 
+  step_bb (instr (push ro) is) (st rf p s h) sn
+  | step_pop : ∀ rf p s h wo is w s' sn,
+  write wo w (st rf p s h) s' → 
+  step_bb is s' sn →
+  step_bb (instr (pop wo) is) (st rf p (w::s) h) sn
+  | step_new : ∀ rf p s h wo is w s' n sn,
+  write wo w (st rf p s h) s' →
+  (∀ i, i < n → not (In (w+i) (domain h))) →
+  step_bb is s' sn → 
+  step_bb (instr (new n wo) is) (st rf p s h) sn 
+  | step_mov : ∀ s is ro wo s' v sn, 
+  read ro s v → write wo v s s' → 
+  step_bb is s' sn → 
+  step_bb (instr (mov ro wo) is) s sn
+  | step_jump0 : ∀ ro k j s s', 
+  read ro s 0 →
+  write (WR IP) k s s' → 
+  step_bb (jump (Some (ro, k)) j) s s'
+.
+
+Inductive step : transition State :=
+  | enter : ∀ rf p s h k bb sn,
+    read IP (st rf p s h) k → 
+    nth k p bb → 
+    step_bb bb (st rf p s h) sn →
+    step (st rf p s h) sn.
 
