cem_cesm.v
@@ -1,43 +1,43 @@
-Require Import cem cesm.
+Require Import cem cesm relations List.
 Require Import Unicode.Utf8.
-Require Import relations. 
-Require Import List. 
+Require cem.
 
-Notation " c1 '→_s*' c2 " := (refl_trans_clos step' c1 c2) (at level 30). 
+Notation " c1 '→_s*' c2 " := (refl_trans_clos cesm_step c1 c2) (at level 30). 
 
 Definition b2s (c : configuration) : stack → state := match c with
   | conf h c => λ s, st h s c end.
 
-Definition convert_to_cesm (c c' : configuration) : Prop := match (c, c') with
+Definition convert_to_cesm (c c' : configuration) : Type := match (c, c') with
   | (conf h c, conf h' c') => ∀ s, (st h s c) →_s* (st h' s c') end.
 
 Lemma cem_cesm : ∀ c v, c ⇓ v → ∀ s, b2s c s →_s* b2s v s. 
+intros c v H. induction H.
 (* Var *)
-intros c v H. induction H. simpl. simpl in IHstep. 
-assert (∀ s, step' (st (Υ ++ (x ↦ {M,y} :: Φ)) s (close (db.var v) z)) 
-                   (st (Υ ++ (x ↦ {M,y} :: Φ)) (inr x::s) M)).
-intros. apply Var. assumption. 
-assert (∀ s, step' (st (Υ ++ x ↦ {M, y} :: Ψ) (inr x :: s) (close (db.lam B) e))
-                   (st (Υ ++ x ↦ {close (db.lam B) e, y} :: Ψ) s (close (db.lam B) e)))
-.
-apply Upd. 
-intros. rename y into Y.  
-apply t_step with (y:=[Υ ++ x ↦ {M, Y} :: Φ, inr x :: s]M). auto. 
-apply t_step2 with (y:= [Υ ++ x ↦ {M, Y} :: Ψ, inr x :: s](close (db.lam B) e)). 
-auto. auto.   
+- simpl. simpl in IHstep. intros. rename y into Y.  
+  apply t_step with (y:=[Υ ++ x ↦ {M, Y} :: Φ, inr x :: s]M). auto. 
+  + apply Var. assumption. 
+  + apply t_step2 with (y:= [Υ ++ x ↦ {M, Y} :: Ψ, inr x :: s](close (db.lam B) e)). 
+    * apply Upd. 
+    * auto. 
 (* Lam *)
-intros. apply t_refl. 
+- intros. apply t_refl. 
 (* App *)
-intros. apply t_step with (y:=b2s (⟨Φ ⟩ close M e) (inl (close N e)::s)). 
-apply App. 
-apply refl_trans_clos_app with (y:=b2s (⟨Ψ, f ↦ {close N e, ne} ⟩ close B f) s).
-apply t_step2 with (y:=b2s (⟨Ψ ⟩ close (db.lam B) ne) (inl (close N e):: s)).
-simpl. rename e into E. rename s into S. apply Abs with (b:=B) (e:=ne)
-(c:=close N E) (s:= S) in H.  
-assumption.
-auto. 
-auto. 
+- intros. apply t_step with (y:=b2s (⟨Φ ⟩ close M e) (inl (close N e)::s)). 
+  + apply App. 
+  + apply refl_trans_clos_app with (y:=b2s (⟨Ψ, f ↦ {close N e, ne} ⟩ close B f) s).
+    * apply t_step2 with (y:=b2s (⟨Ψ ⟩ close (db.lam B) ne) (inl (close N e):: s)).
+      -- simpl. rename e into E. rename s into S. 
+         apply Abs with (b:=B) (e:=ne) (c:=close N E) (s:= S). 
+         assumption. 
+      -- auto. 
+    * auto. 
 Qed. 
+
+(*
+Lemma cem_cesm_time : ∀ c v (e:c ⇓ v) s, 
+  sigT (fun x => time_cost (b2s c s) (b2s v s) x = cem.time_cost e). 
+induction e.  
+- intros s. simpl in IHe.  
 
 Definition s2b (s : state) : configuration := match s with
   | st h s c => conf h c
@@ -48,7 +48,6 @@ Definition st_stack := λ s, match s with
   end.
 
 
-(*
 Lemma cesm_cem : ∀ c c' v, c →_s c' → c' →_s* v → st_stack c = st_stack v → s2b c ⇓ s2b v.
 intros. induction H0. induction H. simpl in H1. inversion v. induction H1. 
 *)
