db_assembly.v
@@ -1,6 +1,42 @@
+Require Import List. Import ListNotations. 
+Open Scope list_scope. 
 Require Import db assembly util.
 
+Infix "#" := instr (at level 30, right associativity).
+Fixpoint var_inst (i : nat) : BasicBlock := match i with
+  | 0 => push EP #
+         push (RC 0) #
+         mov (EP%0) R1 #
+         mov (EP%1) EP #
+         jump None R1
+  | S i => mov EP (EP%2) # 
+           var_inst i
+  end.
+
+
 (* Assembles deBruijn indices to instructions *)
-Fixpoint assemble (t : tm) : Program.
-Admitted.
-  
+Fixpoint assemble (t : tm) (k : nat) : Program := match t with  
+  | var v => [var_inst v]
+  | app m n => let ms := assemble m (k+1) in
+               let nk := k + 1 + length ms in
+                push EP #
+                push (RC nk) #
+                jump None (RC (k+1)) :: 
+                ms ++ 
+                assemble n nk
+  | lam b => pop R1 #
+             jump (Some (RW (WR R1), (k+1))) (RC (k+2)) ::
+             (*Update*)
+             pop R1 #  
+             mov (RC k) (R1%0) #
+             mov EP (R1%1) #
+             jump None (RC k) ::
+             (*Take*)
+             new 3 R2 #
+             mov R1 (R2%0)#
+             pop (R2%1) #
+             mov EP (R2%2) #
+             mov R2 EP #
+             jump None (k+3) :: nil
+  end. 
+
