relations.v
@@ -1,13 +1,14 @@
 Require Import Unicode.Utf8. 
 
-Definition relation (X : Type) (Y : Type) := X → Y → Prop.
+Open Scope type_scope. 
+Definition relation (X : Type) (Y : Type) := X → Y → Type.
 
-Definition transition (X : Type) := X → X → Prop.
+Definition transition (X : Type) := X → X → Type.
 
 Definition strong_bisim (A B : Type) (fa : transition A) (fb : transition B) (R : relation A B) :
-  Prop := ∀ a b, R a b → 
-          (∀ a', fa a a' → ∃ b', fb b b' ∧ R a' b')
-        ∧ (∀ b', fb b b' → ∃ a', fa a a' ∧ R a' b'). 
+  Type := ∀ a b, R a b → 
+         (∀ a', fa a a' → {b' : B & fb b b' * R a' b'})
+       * (∀ b', fb b b' → {a' : A & fa a a' * R a' b'}). 
 
 Inductive refl_trans_clos {X} (f : transition X) : transition X := 
   | t_refl (x : X) : refl_trans_clos f x x
@@ -15,12 +16,12 @@ Inductive refl_trans_clos {X} (f : transition X) : transition X :=
 
 Lemma t_step2 {X} : ∀ (f : transition X) (x y z : X), f y z → refl_trans_clos f x y →
   refl_trans_clos f x z. 
-intros. induction H0. apply t_step with (y:=z). assumption. apply t_refl. apply
+intros f x y z H H0. induction H0. apply t_step with (y:=z). assumption. apply t_refl. apply
 IHrefl_trans_clos in H. apply (t_step f x y z); assumption. Qed. 
 
 Lemma refl_trans_clos_app {X} : ∀ (f : transition X) (x y z : X), 
   refl_trans_clos f x y → refl_trans_clos f y z → refl_trans_clos f x z. 
-intros. induction H. auto. apply IHrefl_trans_clos in H0. rename y into Y. apply
+intros f x y z H H0. induction H. auto. apply IHrefl_trans_clos in H0. rename y into Y. apply
 t_step with (y:=Y); auto. Qed. 
 
 (* p and q are bisimilar *)
@@ -30,16 +31,16 @@ Definition partial_function {X Y: Type} (R: relation X Y) :=
   ∀ (x : X) (y1 y2 : Y), R x y1 → R x y2 → y1 = y2. 
 
 Definition total_function {X Y: Type} (R: relation X Y) :=
-  (∀ x:X, ∃ y:Y, R x y) ∧ partial_function R. 
+  (∀ x:X, {y:Y & R x y}) * partial_function R. 
 
-Definition surjective {X Y: Type} (f : X → Y) : Prop :=
+Definition surjective {X Y: Type} (f : X → Y) : Type :=
   ∀ y:Y, ∃ x:X, f x = y.
 
-Definition injective {X Y : Type} (f : X → Y) : Prop :=
+Definition injective {X Y : Type} (f : X → Y) : Type :=
   ∀ a b: X, f a = f b → a = b.
 
-Definition bijective {X Y : Type} (f : X → Y) : Prop :=
-  injective f ∧ surjective f.
+Definition bijective {X Y : Type} (f : X → Y) : Type :=
+  injective f * surjective f.
 
 Definition reflexive {X : Type} (R: relation X X) :=
   ∀ a : X, R a a.
@@ -54,16 +55,17 @@ Definition transitive {X: Type} (R: relation X X) :=
   ∀ a b c : X, (R a b) → (R b c) → (R a c).
 
 Definition equivalence {X:Type} (R: relation X X) :=
-  (reflexive R) ∧ (symmetric R) ∧ (transitive R).
+  reflexive R * symmetric R * transitive R.
 
 Definition partial_order {X:Type} (R: relation X X) :=
-  (reflexive R) ∧ (antisymmetric R) ∧ (transitive R).
+  reflexive R * antisymmetric R * transitive R.
 
 (* Examples *)
 
 Inductive next_nat (n : nat) : nat → Prop := 
     | succ : next_nat n (S n).
 
+(*
 Lemma next_nat_le : ∀ m n, refl_trans_clos next_nat m n ↔ le m n.
 intros. split. intros. induction H. auto. inversion H. subst. apply le_S in
 IHrefl_trans_clos. apply le_S_n. assumption. intros. induction H. apply t_refl.
@@ -74,4 +76,4 @@ Theorem bisim_next_nat_eq : strong_bisim nat nat next_nat next_nat eq.
 Proof. unfold strong_bisim. intros. subst. split. intros. apply ex_intro with a'.
 split; auto. intros. apply ex_intro with b'. split; auto. Qed. 
 
-
+*)
